add regression test that triggers bug

silveroak-opentitan/hmac/Spec/Tests/SHA256TestVectors.v
@@ -140,3 +140,9 @@ Definition test2 : sha256_step_by_step_test :=
 Definition test3 : sha256_test_vector :=
   {| msg := N_to_string (64+34) 0x36373435323330313E3F3C3D3A3B383926272425222320212E2F2C2D2A2B282916171415121310111E1F1C1D1A1B181906070405020300010E0F0C0D0A0B080953616D706C65206D65737361676520666F72206B65796C656E3D626C6F636B6C656E;
      expected_digest := 0xC0918E14C43562B910DB4B8101CF8812C3DA2783C670BFF34D88B3B88E731716 |}.
+
+(* Regression test : checks that padder correctly handles the case where there
+   is exactly one word between message and length (52 characters)  *)
+Definition test4 : sha256_test_vector :=
+  {| msg := "abcdefghijklmnopqrstuvwzyzabcdefghijklmnopqrstuvwxyz";
+     expected_digest := 0x8794B1A351873E838EE68D51098C279E9F50ABF5D8B8CBABE97EA3BEA57C6EC7 |}.
